Proving map code generator

Compiler/CompilerProof.v
@@ -1,5 +1,5 @@
 Require Import LibTactics assertion_lemmas GPUCSL TypedTerm Monad
-        Host DepList CUDALib CSLLemma CSLTactics CodeGen Compiler mkMap mkReduce
+        Host DepList CUDALib CSLLemma CSLTactics CodeGen Compiler Skel_lemma mkMap mkReduce
         Correctness CodeGenM SeqCompilerProof Program.
 
 Definition main_spec GA :=
@@ -65,12 +65,146 @@ Proof.
   intros n; destruct p; simpl; rewrite !app_length, !flatTup_length, (IHGA _ (S n)); eauto.
 Qed.
 
+Lemma evalExpseq_cons2 x v E es vs :
+  evalExpseq E es vs
+  -> evalExpseq (x |-> v :: E) es vs .
+Proof.
+  induction 1; constructor; eauto.
+  apply evalExp_cons_ig; eauto.
+Qed.
+
+Lemma evalExpseq_cons E e v es vs :
+  evalExp E e v -> evalExpseq E es vs -> evalExpseq E (e :: es) (v :: vs).
+Proof. constructor; eauto. Qed.
+
+Lemma evalExpseq_flatTupxs E ty (xs : vars ty) vs :
+  incl (xs |=> vs) E
+  -> evalExpseq E (map Evar (flatTup xs)) (flatTup vs).
+Proof.
+  induction ty; simpl; [do 2 constructor; apply H; simpl; eauto..|].
+  intros.
+  rewrite map_app; apply evalExpseq_app; [apply IHty1 | apply IHty2];
+  unfold incl in *; intros x ?; forwards*: (>>H x); rewrite in_app_iff; eauto.
+Qed.
+
+Lemma evalExpseq_app1 E1 E2 es vs :
+  evalExpseq E1 es vs -> evalExpseq (E1 ++ E2) es vs.
+Proof.
+  induction 1; try constructor; eauto.
+  apply evalExp_app1; eauto.
+Qed.
+Lemma evalExp_app2 E1 E2 e v :
+  evalExp E2 e v -> evalExp (E1 ++ E2) e v.
+Proof.
+  induction 1; constructor; eauto.
+  rewrite in_app_iff; eauto.
+Qed.
+
+Lemma evalExpseq_app2 E1 E2 es vs :
+  evalExpseq E2 es vs -> evalExpseq (E1 ++ E2) es vs.
+Proof.
+  induction 1; try constructor; eauto.
+  apply evalExp_app2; eauto.
+Qed.
+
+Fixpoint flatten_aeenv {GA} (aeenv : AEvalEnv GA) : APtrEnv GA -> list val :=
+  match aeenv with
+  | HNil => fun _ => nil
+  | l ::: aeenv => fun apenv =>
+    match apenv in hlist _ GA return (match GA with
+                                      | nil => Empty_set -> list val
+                                      | _ :: GA' => (APtrEnv GA' -> list val) -> list val
+                                      end) with 
+    | HNil => fun none => match none with end
+    | p ::: apenv => fun rec => SkelLib.len l :: flatTup p ++ rec apenv
+    end (flatten_aeenv aeenv)
+  end%list.
+
+Lemma evalExpseq_arrInv GA (avenv : AVarEnv GA) apenv aeenv :
+  evalExpseq (arrInvVar avenv apenv aeenv) (map Evar (flatten_aenv avenv)) (flatten_aeenv aeenv apenv).
+Proof.
+  unfold arrInvVar; induction GA; 
+  dependent destruction avenv; dependent destruction apenv; dependent destruction aeenv; simpl.
+  constructor.
+  destruct p; simpl.
+  apply evalExpseq_cons; [evalExp|].
+  rewrite map_app.
+  apply evalExpseq_cons2.
+  apply evalExpseq_app.
+  - apply evalExpseq_app1.
+    applys* evalExpseq_flatTupxs.
+  - applys* evalExpseq_app2.
+Qed.
+
+Lemma out_name_locals typ :
+  map fst (flatTup (out_name typ)) = flatTup (mkMap.outArr typ).
+Proof.
+  unfold out_name, mkMap.outArr; generalize 0.
+  induction typ; simpl; eauto.
+  intros; rewrite map_app, IHtyp1, IHtyp2; eauto.
+Qed.
+
+Lemma subst_env_app E1 E2 xs vs : 
+  subst_env (E1 ++ E2) xs vs <-> (subst_env E1 xs vs /\ subst_env E2 xs vs)%list.
+Proof.
+  induction E1 as [|[? ?] ?]; simpl; tauto.
+Qed.
+
+Lemma subst_env_cons2 E x xs v vs :
+  ~In x (map ent_e E)
+  -> subst_env E xs vs
+  -> subst_env E (x :: xs) (v :: vs).
+Proof.
+  induction E as [|[? ?] ?]; simpl; eauto.
+  destruct var_eq_dec; substs; try tauto.
+Qed.
+
+Lemma subst_env_app1 E xs1 xs2 vs1 vs2 :
+  subst_env E xs1 vs1
+  -> subst_env E (xs1 ++ xs2) (vs1 ++ vs2).
+Proof.
+  induction E as [|[? ?] ?]; simpl; eauto.
+  intros [? ?]; split; eauto.
+  revert H; clear; revert xs2 vs1 vs2; clear.
+  induction xs1; simpl; intros; try tauto.
+  destruct vs1; try tauto.
+  destruct var_eq_dec; substs; simpl; eauto.
+Qed.
+
+Lemma subst_env_app2 E xs1 xs2 vs1 vs2 :
+  length xs1 = length vs1
+  -> disjoint (map ent_e E) xs1
+  -> subst_env E xs2 vs2
+  -> subst_env E (xs1 ++ xs2) (vs1 ++ vs2).
+Proof.
+  induction E as [|[? ?] ?]; simpl; eauto.
+  intros Hlen [? ?] [? ?]; split; eauto.
+  revert Hlen H H1; clear; revert xs2 vs1 vs2.
+  induction xs1; simpl; introv; destruct vs1; simpl; try congruence; eauto.
+  intros Heq Hdis Hsubst; destruct var_eq_dec; try tauto; eauto.
+Qed.
+
+Lemma subst_env_flatTup typ (xs : vars typ) vs :
+  disjoint_list (flatTup xs)
+  -> subst_env (xs |=> vs) (flatTup xs) (flatTup vs).
+Proof.
+  induction typ; simpl; [destruct var_eq_dec; tauto..|].
+  intros Hdisj.
+  apply subst_env_app; split.
+  apply subst_env_app1; eauto using disjoint_list_proj1.
+  apply subst_env_app2; [repeat rewrites* flatTup_length|..].
+  apply disjoint_list_app_disjoint in Hdisj.
+  rewrite map_flatTup; eauto using disjoint_comm.
+  apply IHtyp2; eauto using disjoint_list_proj2.
+Qed.
+
 Lemma compile_map_ok GA dom cod ntrd nblk
       (avenv : AVarEnv GA) (apenv : APtrEnv GA) (aeenv : AEvalEnv GA)
       (f : Skel.Func GA (Skel.Fun1 dom cod))
       (arr : Skel.AE GA dom) (result : Skel.aTypDenote cod)
       xs fns Gp :
-  Skel.skelDenote GA cod (Skel.Map GA dom cod f arr) aeenv = Some result
+  ntrd <> 0 -> nblk <> 0
+  -> Skel.skelDenote GA cod (Skel.Map GA dom cod f arr) aeenv = Some result
   -> ST_ok (preST xs fns (kernelInv avenv apenv aeenv Emp True nil 1) Gp)
            (compile_map ntrd nblk avenv f arr)
            (fun res => postST xs fns (kernelInv avenv apenv aeenv Emp True nil 1)
@@ -79,7 +213,7 @@ Lemma compile_map_ok GA dom cod ntrd nblk
                                                     True
                                                     (fst res |-> len :: snd res |=> ps) 1%Qc) Gp nil).
 Proof.
-  intros Heval.
+  intros Hntrd0 Hnblk0 Heval.
 
   unfold Skel.skelDenote in Heval.
   unfold bind in Heval; simpl in Heval.
@@ -125,13 +259,46 @@ Proof.
       do 2 f_equal.
       rewrite flatten_aenv_avars_length; eauto.
     - repeat econstructor.
-    - do 3 (constructor; [evalExp|]).
-      rewrite map_app.
-
-      apply Forall2_app.
+    - do 3 (apply evalExpseq_cons; [evalExp|]).
+      simpl; rewrite map_app; apply evalExpseq_app.
+      apply evalExpseq_app1.
+      apply evalExpseq_flatTupxs; eauto.
+      apply evalExpseq_app2, evalExpseq_cons2.
+      apply evalExpseq_arrInv.
+    - eauto.
+    - eauto.
+    - simpl.
+      rewrite !map_app.
+      intros [? ?]; splits; eauto.
+      + unfold mkMap.arr_res.
+        destruct mkMap.eval_arr_ok.
+        rewrite Heq1 in e; inverts e; eauto.
+      + rewrite subst_env_app; split.
+        * unfold mkMap.outArr.
+          repeat (apply subst_env_cons2; [rewrite map_flatTup; apply locals_not_in; simpl; eauto|]).  
+          apply subst_env_app1.
+          rewrite out_name_locals.
+          apply subst_env_flatTup; apply locals_disjoint_ls.
+        * instantiate (1 := apenv).
+          skip. 
+    - intros [? ?]; splits; eauto.
       
-      Lemma 
-
+      skip. skip.
+      instantiate (1 := result).
+      instantiate (1 := vs).
+      forwards*: SkelLib.mapM_length; congruence.
+    - intros; rewrite <-res_assoc.
+      repeat sep_cancel'.
+      eauto. }
+  introv.
+  Lemma rule_ret_ignore (T : Type) P (v : T) Q : ST_ok P (ret v) (fun _ => Q).
+                                                   admit.
+  Qed.
+  instantiate (1 := (fun _ _ => True)).
+  instantiate (1 := K (K fns)).
+  instantiate (1 := K (K xs)).
+  unfold K.
+  apply (rule_ret_ignore _ _ (outLen, outs) (fun _ => _)).
 
 Theorem compile_AS_ok GA ty ntrd nblk (p : Skel.AS GA ty) :
   let M := compile_prog ntrd nblk p in
